DynamoDbEncryption/runtimes/java/src/main/smithy-generated/software/amazon/cryptography/dynamoDbEncryption/ToNative.java
@@ -109,6 +109,7 @@ public class ToNative {
   public static DynamoDbTableEncryptionConfig DynamoDbTableEncryptionConfig(
       Dafny.Aws.Cryptography.DynamoDbEncryption.Types.DynamoDbTableEncryptionConfig dafnyValue) {
     DynamoDbTableEncryptionConfig.Builder nativeBuilder = DynamoDbTableEncryptionConfig.builder();
+    nativeBuilder.logicalTableName(software.amazon.dafny.conversion.ToNative.Simple.String(dafnyValue.dtor_logicalTableName()));
     nativeBuilder.partitionKeyName(software.amazon.dafny.conversion.ToNative.Simple.String(dafnyValue.dtor_partitionKeyName()));
     if (dafnyValue.dtor_sortKeyName().is_Some()) {
       nativeBuilder.sortKeyName(software.amazon.dafny.conversion.ToNative.Simple.String(dafnyValue.dtor_sortKeyName().dtor_value()));
