DynamoDbEncryption/dafny/DynamoDbEncryptionTransforms/src/Index.dfy
@@ -75,8 +75,42 @@ module
     || (config.allowedUnauthenticatedAttributePrefix.Some? && config.allowedUnauthenticatedAttributePrefix.value <= name)
   }
 
+  predicate {:opaque} AllTableConfigsValid?(configs: map<string, TableConfig>)
+    ensures 0 == |configs| ==> AllTableConfigsValid?(configs)
+  {
+    forall tableName <- configs :: ValidTableConfig?(configs[tableName])
+  }
+  predicate {:opaque} CorrectlyTransferedStructure?(
+    internalConfigs: map<string, DdbMiddlewareConfig.ValidTableConfig>,
+    config: AwsCryptographyDynamoDbEncryptionTypes.DynamoDbTablesEncryptionConfig
+  )
+    ensures 0 == |internalConfigs| ==> CorrectlyTransferedStructure?(internalConfigs, config)
+  {
+    forall tableName <- internalConfigs
+    ::
+      && tableName in config.tableEncryptionConfigs
+      && ConfigsMatch(tableName, internalConfigs[tableName], config.tableEncryptionConfigs[tableName])
+  }
+  predicate {:opaque} ConfigsMatch(
+    tableName: string,
+    internalConfig: DdbMiddlewareConfig.ValidTableConfig,
+    inputConfig: AwsCryptographyDynamoDbEncryptionTypes.DynamoDbTableEncryptionConfig
+  )
+  {
+    && tableName == internalConfig.physicalTableName
+    && inputConfig.logicalTableName == internalConfig.logicalTableName
+    && inputConfig.partitionKeyName == internalConfig.partitionKeyName
+    && inputConfig.sortKeyName == internalConfig.sortKeyName
+  }
+
   method {:vcs_split_on_every_assert} DynamoDbEncryptionTransforms(config: AwsCryptographyDynamoDbEncryptionTypes.DynamoDbTablesEncryptionConfig)
     returns (res: Result<DynamoDbEncryptionTransformsClient, Error>)
+      //= specification/dynamodb-encryption-client/ddb-table-encryption-config.md#logical-table-name
+      //= type=implication
+      //# When mapping [DynamoDB Table Names](#dynamodb-table-name) to [logical table name](#logical-table-name)
+      //# there MUST a one to one mapping between the two.
+      ensures res.Success? ==>
+        && DdbMiddlewareConfig.ValidConfig?(res.value.config)
   {
     var internalConfigs: map<string, DdbMiddlewareConfig.ValidTableConfig> := map[];
     assert ValidWholeSearchConfig(config);
@@ -85,28 +119,33 @@ module
     //# [DynamoDb Item Encryptor](./ddb-table-encryption-config.md)
     //# per configured table, using these table encryption configs.
     var m' := config.tableEncryptionConfigs;
+
+    ghost var inputConfigsModifies: set<object> := set
+      tableConfig <- config.tableEncryptionConfigs.Values,
+      o <- (
+            (if tableConfig.keyring.Some? then tableConfig.keyring.value.Modifies else {})
+          + (if tableConfig.cmm.Some? then tableConfig.cmm.value.Modifies else {})
+          + (if tableConfig.legacyConfig.Some? then tableConfig.legacyConfig.value.encryptor.Modifies else {})
+      )
+      :: o;
+
+    var allLogicalTableNames := {};
+
     while m'.Keys != {}
         invariant m'.Keys <= config.tableEncryptionConfigs.Keys
         invariant forall k <- m' :: m'[k] == config.tableEncryptionConfigs[k]
-        invariant forall k <- internalConfigs :: OneSearchValidState(internalConfigs[k])
-        invariant forall tableName <- internalConfigs, tableConfig :: (tableConfig == internalConfigs[tableName]
-          ==>
-            && tableConfig.itemEncryptor.config.tableName == tableName
-            && tableConfig.itemEncryptor.config.partitionKeyName == tableConfig.partitionKeyName
-            && tableConfig.itemEncryptor.config.sortKeyName == tableConfig.sortKeyName)
-        invariant forall t :: t in internalConfigs.Keys ==> internalConfigs[t].itemEncryptor.ValidState()
+        invariant forall internalConfig <- internalConfigs.Values :: internalConfig.logicalTableName in allLogicalTableNames
 
-        invariant fresh((set t <- internalConfigs.Keys, o <- internalConfigs[t].itemEncryptor.Modifies :: o) -
-          set t <- config.tableEncryptionConfigs.Keys, o <- (
-            (if config.tableEncryptionConfigs[t].keyring.Some? then config.tableEncryptionConfigs[t].keyring.value.Modifies else {})
-          + (if config.tableEncryptionConfigs[t].cmm.Some? then config.tableEncryptionConfigs[t].cmm.value.Modifies else {})
-          + (if config.tableEncryptionConfigs[t].legacyConfig.Some? then config.tableEncryptionConfigs[t].legacyConfig.value.encryptor.Modifies else {})
-      ) :: o)
+        invariant CorrectlyTransferedStructure?(internalConfigs, config)
+        invariant AllTableConfigsValid?(internalConfigs)
+        invariant ValidConfig?(Config(internalConfigs))
 
         decreases m'.Keys
+        modifies inputConfigsModifies
     {
         var tableName: string :| tableName in m';
         var inputConfig := config.tableEncryptionConfigs[tableName];
+        :- Need(inputConfig.logicalTableName !in allLogicalTableNames,  E("Duplicate logical table maped to multipule physical tables: " + inputConfig.logicalTableName));
 
         assert SearchConfigToInfo.ValidSearchConfig(inputConfig.search);
         SearchInModifies(config, tableName);
@@ -131,7 +170,7 @@ module
         var newActions := AddSignedBeaconActions(signedBeacons, inputConfig.attributeActions);
 
         var encryptorConfig := AwsCryptographyDynamoDbEncryptionItemEncryptorTypes.DynamoDbItemEncryptorConfig(
-          tableName := tableName,
+          logicalTableName := inputConfig.logicalTableName,
           partitionKeyName := inputConfig.partitionKeyName,
           sortKeyName := inputConfig.sortKeyName,
           attributeActions := newActions,
@@ -143,31 +182,55 @@ module
           legacyConfig := inputConfig.legacyConfig,
           plaintextPolicy := inputConfig.plaintextPolicy
         );
+
         // TODO consider using the raw constructor in order to avoid
         // instantiating multiple StructuredEncryption
         var itemEncryptorRes := DynamoDbItemEncryptor.DynamoDbItemEncryptor(encryptorConfig);
-
         var itemEncryptor :- itemEncryptorRes
           .MapFailure(e => AwsCryptographyDynamoDbEncryptionItemEncryptor(e));
-        var internalConfig := DdbMiddlewareConfig.TableConfig(
+
+        var internalConfig: DdbMiddlewareConfig.ValidTableConfig := DdbMiddlewareConfig.TableConfig(
+          physicalTableName := tableName,
+          logicalTableName := inputConfig.logicalTableName,
           partitionKeyName := inputConfig.partitionKeyName,
           sortKeyName := inputConfig.sortKeyName,
           itemEncryptor := itemEncryptor,
           search := search
         );
-        assert OneSearchValidState(internalConfig);
-        assert internalConfig.itemEncryptor.ValidState();
+        
         internalConfigs := internalConfigs[tableName := internalConfig];
-        assert forall k <- internalConfigs :: OneSearchValidState(internalConfigs[k]);
+        allLogicalTableNames := allLogicalTableNames + {internalConfig.logicalTableName};
+
+        assert AllTableConfigsValid?(internalConfigs) by {
+          reveal AllTableConfigsValid?();
+          assert AllTableConfigsValid?(internalConfigs - {tableName});
+          assert ValidTableConfig?(internalConfig);
+        }
+        assert ValidConfig?(Config(internalConfigs)) by {
+          assert ValidConfig?(Config(internalConfigs - {tableName}));
+          assert internalConfig.physicalTableName == tableName;
+        }
+
+        assert CorrectlyTransferedStructure?(internalConfigs, config) by {
+          reveal CorrectlyTransferedStructure?();
+          reveal ConfigsMatch();
+          assert CorrectlyTransferedStructure?(internalConfigs - {tableName}, config);
+          assert ConfigsMatch(tableName, internalConfig, inputConfig);
+        }
 
         // Pop 'tableName' off the map, so that we may continue iterating
         m' := map k' | k' in m' && k' != tableName :: m'[k'];
     }
     assert SearchValidState(DdbMiddlewareConfig.Config(tableEncryptionConfigs := internalConfigs));
+
+    var newConfig := DdbMiddlewareConfig.Config(tableEncryptionConfigs := internalConfigs);
+    assert Operations.ValidInternalConfig?(newConfig);
+    var client := new DynamoDbEncryptionTransformsClient(newConfig);
+
     // I'm really sorry, but I can't get the freshness to verify
     // and my time box has run out of time.
     assume {:axiom} fresh(
-     Operations.ModifiesInternalConfig(DdbMiddlewareConfig.Config(tableEncryptionConfigs := internalConfigs))
+      client.Modifies
         - ( var tmps14 := set t14 | t14 in config.tableEncryptionConfigs.Values
           && t14.keyring.Some? 
           :: t14.keyring.value;
@@ -205,18 +268,6 @@ module
         && tmp22ModifyEntry in tmp22Modifies 
         :: tmp22ModifyEntry)
         ) );
-
-    assert forall tableName <- internalConfigs ::
-      var tableConfig := internalConfigs[tableName];
-      && tableConfig.itemEncryptor.config.tableName == tableName
-      && tableConfig.itemEncryptor.config.partitionKeyName == tableConfig.partitionKeyName
-      && tableConfig.itemEncryptor.config.sortKeyName == tableConfig.sortKeyName
-      && tableConfig.itemEncryptor.ValidState()
-      && OneSearchValidState(tableConfig);
-
-    var newConfig := DdbMiddlewareConfig.Config(tableEncryptionConfigs := internalConfigs);
-    assert Operations.ValidInternalConfig?(newConfig);
-    var client := new DynamoDbEncryptionTransformsClient(newConfig);
 
     return Success(client);
   }
