DynamoDbEncryption/dafny/DynamoDbItemEncryptor/Model/AwsCryptographyDynamoDbEncryptionItemEncryptorTypes.dfy
@@ -94,7 +94,7 @@ include "../../../../submodules/MaterialProviders/StandardLibrary/src/Index.dfy"
  
 }
  datatype DynamoDbItemEncryptorConfig = | DynamoDbItemEncryptorConfig (
- nameonly tableName: ComAmazonawsDynamodbTypes.TableName ,
+ nameonly logicalTableName: string ,
  nameonly partitionKeyName: ComAmazonawsDynamodbTypes.KeySchemaAttributeName ,
  nameonly sortKeyName: Option<ComAmazonawsDynamodbTypes.KeySchemaAttributeName> ,
  nameonly attributeActions: AwsCryptographyDynamoDbEncryptionTypes.AttributeActions ,
